move Jensen's inequalities to core theories

src/real/transcScript.sml
@@ -36,6 +36,7 @@ open hol88Lib
      PairedLambda
      jrhUtils
      Diff
+     pred_setTheory
      mesonLib
      RealArith;
 
@@ -4150,16 +4151,198 @@ Proof
       REAL_ARITH_TAC ] ]
 QED
 
+(* ------------------------------------------------------------------------- *)
+(* ----------- exp is a convex function (from "miller" example) ------------ *)
+(* ------------------------------------------------------------------------- *)
+
+val Suff = Q_TAC SUFF_TAC;
+val Know = Q_TAC KNOW_TAC;
+
+Definition convex_fn :
+    convex_fn =
+      {f | !x y t. (0 <= t /\ t <= 1) ==>
+                   f (t * x + (1 - t) * y) <= t * f x + (1 - t) * f y}
+End
+
+Definition concave_fn :
+    concave_fn = {f | (\x. ~ (f x)) IN convex_fn}
+End
+
+val exp_convex_lemma1 = prove (
+   ``!t. (t + (1 - t) * exp 0 - exp ((1 - t) * 0) = 0) /\
+         (t * exp 0 + (1 - t) - exp (t * 0) = 0)``,
+   RW_TAC real_ss [EXP_0] >> REAL_ARITH_TAC);
+
+val exp_convex_lemma2 = prove (
+   ``!t x. ((\x. (1 - t) * exp x - exp ((1 - t) * x)) diffl
+            (\x. (1-t) * exp x - (1 - t)*exp ((1-t)*x)) x) x``,
+   RW_TAC std_ss []
+   >> `(\x. (1 - t) * exp x - exp ((1 - t) * x)) =
+       (\x. (\x. (1 - t) * exp x) x - (\x. exp ((1 - t) * x)) x)`
+        by RW_TAC std_ss [FUN_EQ_THM]
+   >> POP_ASSUM (fn thm => ONCE_REWRITE_TAC [thm])
+   >> `((1 - t) * exp x - (1 - t) * exp ((1 - t) * x)) =
+       (\x. (1 - t) * exp x) x - (\x. (1-t) * exp ((1- t) * x)) x`
+        by RW_TAC std_ss []
+   >> POP_ASSUM (fn thm => ONCE_REWRITE_TAC [thm])
+   >> Suff `((\x. (1 - t) * exp x) diffl (\x. (1 - t) * exp x) x) x /\
+                ((\x. exp ((1 - t) * x)) diffl (\x. (1 - t) * exp ((1 - t) * x)) x) x`
+   >- METIS_TAC [DIFF_SUB]
+   >> CONJ_TAC
+   >- (`(\x. (1 - t) * exp x) x = 0 * exp x + (exp x) * (\x. 1 - t) x` by RW_TAC real_ss [REAL_MUL_COMM]
+       >> POP_ASSUM (fn thm => ONCE_REWRITE_TAC [thm])
+       >> Q.ABBREV_TAC `foo = (0 * exp x + exp x * (\x. 1 - t) x)`
+       >> `(\x. (1 - t) * exp x) = (\x. (\x. 1 - t) x * exp x)` by RW_TAC std_ss [FUN_EQ_THM]
+       >> POP_ASSUM (fn thm => ONCE_REWRITE_TAC [thm])
+       >> Q.UNABBREV_TAC `foo`
+       >> MATCH_MP_TAC DIFF_MUL
+       >> RW_TAC std_ss [DIFF_CONST, DIFF_EXP])
+   >> `(\x. exp ((1 - t) * x)) = (\x. exp ((\x. (1-t)*x) x))` by RW_TAC std_ss [FUN_EQ_THM]
+   >> POP_ASSUM (fn thm => ONCE_REWRITE_TAC [thm])
+   >> `(\x. (1 - t) * exp ((1 - t) * x)) x = exp ((\x. (1-t)*x) x) * (1-t)`
+        by RW_TAC real_ss [REAL_MUL_COMM]
+   >> POP_ASSUM (fn thm => ONCE_REWRITE_TAC [thm])
+   >> Suff `((\x. (1 - t) * x) diffl (1-t)) x` >- METIS_TAC [DIFF_COMPOSITE]
+   >> `(1 - t) = (1 - t) * 1` by RW_TAC real_ss []
+   >> POP_ASSUM (fn thm => ONCE_REWRITE_TAC [thm])
+   >> `(\x. (1 - t) * 1 * x) = (\x. (1-t) * (\x. x) x)` by RW_TAC real_ss [FUN_EQ_THM]
+   >> POP_ASSUM (fn thm => ONCE_REWRITE_TAC [thm])
+   >> MATCH_MP_TAC DIFF_CMUL
+   >> RW_TAC std_ss [DIFF_X]);
+
+val exp_convex_lemma3 = prove (
+   ``!t x. (\x. (1-t) * exp x - exp ((1-t)*x)) contl x``,
+   METIS_TAC [DIFF_CONT, exp_convex_lemma2]);
+
+val exp_convex_lemma4 = prove (
+   ``!x. 0 < x /\ 0 < t /\ t < 1 ==> 0 < (\x. (1-t) * exp x - (1 - t)*exp ((1-t)*x)) x``,
+   RW_TAC real_ss [REAL_LT_SUB_LADD] >> MATCH_MP_TAC REAL_LT_LMUL_IMP
+   >> RW_TAC real_ss [REAL_LT_SUB_LADD, EXP_MONO_LT, REAL_SUB_RDISTRIB]
+   >> RW_TAC real_ss [REAL_LT_SUB_RADD, REAL_LT_ADDR] >> MATCH_MP_TAC REAL_LT_MUL
+   >> RW_TAC real_ss []);
+
+val exp_convex_lemma5 = prove (
+   ``!f f' i j. (!x. (f diffl f' x) x) /\
+                (!x. f contl x) /\
+                (0 <= i /\ i < j) /\
+                (!x. i < x /\ x < j ==> 0 < f' x) ==>
+                        f i < f j``,
+   REPEAT STRIP_TAC
+   >> MATCH_MP_TAC REAL_LET_TRANS >> Q.EXISTS_TAC `0 + f i` >> CONJ_TAC >- RW_TAC real_ss []
+   >> RW_TAC real_ss [GSYM REAL_LT_SUB_LADD]
+   >> `?l z. i < z /\ z < j /\ (f diffl l) z /\ (f j - f i = (j - i) * l)`
+        by (MATCH_MP_TAC MVT >> METIS_TAC [differentiable])
+   >> POP_ASSUM (fn thm => ONCE_REWRITE_TAC [thm])
+   >> MATCH_MP_TAC REAL_LT_MUL
+   >> RW_TAC real_ss [REAL_LT_SUB_LADD]
+   >> `l = f' z`
+        by (MATCH_MP_TAC DIFF_UNIQ >> Q.EXISTS_TAC `f` >> Q.EXISTS_TAC `z` >> RW_TAC std_ss [])
+   >> POP_ASSUM (fn thm => ONCE_REWRITE_TAC [thm])
+   >> Q.PAT_X_ASSUM `!x. i < x /\ x < j ==> 0 < f' x` MATCH_MP_TAC >> RW_TAC std_ss []);
+
+val exp_convex_lemma6 = prove (
+   ``!x y t. 0 < t /\ t < 1 /\ x < y ==>
+                exp (t * x + (1 - t) * y) <= t * exp x + (1 - t) * exp y``,
+   REPEAT STRIP_TAC
+   >> Q.ABBREV_TAC `z = y - x`
+   >> `0 < z` by (Q.UNABBREV_TAC `z` >> RW_TAC real_ss [REAL_LT_SUB_LADD])
+   >> Suff `exp (t * x + (1 - t) * (x+z)) <= t * exp x + (1 - t) * exp (x+z)`
+   >- (Q.UNABBREV_TAC `z` >> RW_TAC real_ss [])
+   >> `t * x + (1 - t) * (x + z) = x + (1 - t) * z` by REAL_ARITH_TAC
+   >> ASM_REWRITE_TAC [] >> POP_ASSUM (K ALL_TAC)
+   >> PURE_REWRITE_TAC [EXP_ADD]
+   >> `t * exp x + (1 - t) * (exp x * exp z) = exp x * (t + (1 - t) * exp z)`
+                by REAL_ARITH_TAC
+   >> ASM_REWRITE_TAC [] >> POP_ASSUM (K ALL_TAC)
+   >> MATCH_MP_TAC REAL_LE_LMUL_IMP >> CONJ_TAC >- SIMP_TAC std_ss [EXP_POS_LE]
+   >> MATCH_MP_TAC REAL_LE_TRANS >> Q.EXISTS_TAC `0 + exp ((1 - t) * z)` >> CONJ_TAC >- RW_TAC real_ss []
+   >> ONCE_REWRITE_TAC [GSYM REAL_LE_SUB_LADD]
+   >> MATCH_MP_TAC REAL_LT_IMP_LE
+   >> MATCH_MP_TAC REAL_LET_TRANS >> Q.EXISTS_TAC `t + (1 - t) * exp 0 - exp ((1 - t) * 0)`
+   >> CONJ_TAC >- RW_TAC real_ss [exp_convex_lemma1]
+   >> `t + (1 - t) * exp 0 - exp ((1 - t) * 0) = ((1 - t) * exp 0 - exp ((1 - t) * 0)) + t`
+                by REAL_ARITH_TAC >> ASM_REWRITE_TAC [] >> POP_ASSUM (K ALL_TAC)
+   >> ONCE_REWRITE_TAC [REAL_LT_ADD_SUB]
+   >> `t + (1 - t) * exp z - exp ((1 - t) * z) - t = (1 - t) * exp z - exp ((1 - t) * z)`
+                by REAL_ARITH_TAC
+   >> ASM_REWRITE_TAC [] >> POP_ASSUM (K ALL_TAC)
+   >> Q.ABBREV_TAC `f = (\x. (1-t) * exp x - exp ((1-t)*x))`
+   >> Suff `f 0 < f z` >- (Q.UNABBREV_TAC `f` >> RW_TAC std_ss [])
+   >> MATCH_MP_TAC exp_convex_lemma5
+   >> Q.EXISTS_TAC `(\x. (1-t) * exp x - (1 - t)*exp ((1-t)*x))`
+   >> Q.UNABBREV_TAC `f`
+   >> RW_TAC real_ss [exp_convex_lemma2, exp_convex_lemma3, exp_convex_lemma4]);
+
+val exp_convex = store_thm
+  ("exp_convex",
+   ``exp IN convex_fn``,
+   RW_TAC std_ss [convex_fn, EXTENSION, NOT_IN_EMPTY, GSPECIFICATION]
+   >> Cases_on `t = 0` >- RW_TAC real_ss []
+   >> Cases_on `t = 1` >- RW_TAC real_ss []
+   >> `0 < t /\ t < 1` by METIS_TAC [REAL_LT_LE]
+   >> Cases_on `x = y` >- RW_TAC real_ss []
+   >> (MP_TAC o Q.SPECL [`x`, `y`]) REAL_LT_TOTAL >> RW_TAC std_ss []
+   >- (MATCH_MP_TAC exp_convex_lemma6 >> RW_TAC std_ss [])
+   >> Q.ABBREV_TAC `t' = 1 - t`
+   >> `t = 1 - t'` by (Q.UNABBREV_TAC `t'` >> REAL_ARITH_TAC)
+   >> POP_ASSUM (fn thm => ONCE_REWRITE_TAC [thm])
+   >> `0 < t'` by (Q.UNABBREV_TAC `t'` >> RW_TAC real_ss [REAL_LT_SUB_LADD])
+   >> `t' < 1` by (Q.UNABBREV_TAC `t'` >> RW_TAC real_ss [REAL_LT_SUB_RADD, REAL_LT_ADDR])
+   >> ONCE_REWRITE_TAC [REAL_ADD_COMM]
+   >> MATCH_MP_TAC exp_convex_lemma6 >> RW_TAC std_ss []);
+
+(* ------------------------------------------------------------------------- *)
+(* ------------ ln and lg are concave on (0,infty] ------------------------- *)
+(* ------------------------------------------------------------------------- *)
+
+Definition pos_convex_fn :
+    pos_convex_fn = {f | !x y t. (0 < x /\ 0 < y /\ 0 <= t /\ t <= 1) ==>
+                                 f (t * x + (1 - t) * y) <= t * f x + (1 - t) * f y}
+End
+
+Definition pos_concave_fn :
+    pos_concave_fn = {f | (\x. ~ (f x)) IN pos_convex_fn}
+End
+
+val pos_concave_ln = store_thm
+  ("pos_concave_ln",
+   ``ln IN pos_concave_fn``,
+   RW_TAC std_ss [pos_concave_fn, pos_convex_fn, EXTENSION, NOT_IN_EMPTY, GSPECIFICATION]
+   >> Cases_on `t = 0` >- RW_TAC real_ss []
+   >> Cases_on `t = 1` >- RW_TAC real_ss []
+   >> `0 < t /\ t < 1` by RW_TAC std_ss [REAL_LT_LE]
+   >> `t * ~ln x + (1 - t) * ~ln y = ~ (t * ln x + (1 - t)* ln y)` by REAL_ARITH_TAC
+   >> POP_ASSUM (fn thm => ONCE_REWRITE_TAC [thm])
+   >> RW_TAC std_ss [REAL_LE_NEG, ln]
+   >> MATCH_MP_TAC SELECT_ELIM_THM
+   >> RW_TAC std_ss [] >- (MATCH_MP_TAC EXP_TOTAL
+                           >> MATCH_MP_TAC REAL_LT_ADD >> CONJ_TAC >> MATCH_MP_TAC REAL_LT_MUL
+                           >> RW_TAC real_ss [GSYM REAL_LT_ADD_SUB])
+   >> Suff `(\v. t * v + (1 - t) * (@u. exp u = y) <= x') (@u. exp u = x)`
+   >- RW_TAC std_ss []
+   >> MATCH_MP_TAC SELECT_ELIM_THM
+   >> RW_TAC std_ss [] >- (MATCH_MP_TAC EXP_TOTAL >> RW_TAC std_ss [])
+   >> Suff `(\v. t * x'' + (1 - t) * v <= x') (@u. exp u = y)`
+   >- RW_TAC std_ss []
+   >> MATCH_MP_TAC SELECT_ELIM_THM
+   >> RW_TAC std_ss [] >- (MATCH_MP_TAC EXP_TOTAL >> RW_TAC std_ss [])
+   >> ONCE_REWRITE_TAC [GSYM EXP_MONO_LE]
+   >> POP_ASSUM (fn thm => ONCE_REWRITE_TAC [thm])
+   >> MP_TAC exp_convex >> RW_TAC std_ss [convex_fn, EXTENSION, NOT_IN_EMPTY, GSPECIFICATION]);
+
+(* NOTE: Jensen's inequalities are in real_sigmaScript.sml *)
+
 val _ = Theory.quote_adjoin_to_theory
 `(* val basic_diffs : Thm.thm list ref; *)`
 `local in
   open Diff Drule;
 
-  val _ = basic_diffs := !basic_diffs@[DIFF_EXP, DIFF_SIN, DIFF_COS];
+  val _ = basic_diffs := !basic_diffs@[DIFF_EXP, DIFF_LN];
+  val _ = basic_diffs := !basic_diffs@[DIFF_SIN, DIFF_COS, DIFF_TAN];
+  val _ = basic_diffs := !basic_diffs@[DIFF_ASN, DIFF_ACS, DIFF_ATN];
   val _ = basic_diffs := !basic_diffs@(CONJUNCTS DIFF_COMPOSITE);
-  val _ = basic_diffs := !basic_diffs@[DIFF_LN];
   val _ = basic_diffs := !basic_diffs@[SPEC_ALL DIFF_LN_COMPOSITE];
 end
-`
+`;
 
 val _ = export_theory();
